Fixed the sections so that universal quantification over hash functions works correctly.
Signed-off-by: Andrew Miller <amiller@dappervision.com>

coq/merkle.v
@@ -1,21 +1,7 @@
 Require Import monads.  (* MathClasses library *)
 Require Import monads_. (* monads_.v *)
 
-(* Authenticated Data Structures (Generalized Merkle Trees)
-
-   Tree:   the entire data structure - O(N)
-   VO:     a path through a Tree (i.e., a Verification Object)used 
-           to verify a single operation - O(log N)
-   Digest: a concise representation of a Tree - O(1)
-*)
-
-(* Let HRange be the range of an arbitrary hash function. HRange
-   will be provided by the environment, although the implementation gets 
-   to select the HDomain. Once an HDomain is defined,
-   the implementation must satisfy all the requirements for all possible
-   hash functions from this HDomain. This allows us to express Collisions
-  very generally. *)
-
+(* Authenticated Data Structures (A general form of Merkle trees) *)
 
 (* Define a type of functional maps. *)
 (* TODO: Instantiate this by borrowing from FMap.FMapInterfaces Sord*)
@@ -27,42 +13,40 @@ Parameter search : Map -> k -> option v.
 Parameter insert : Map -> k -> v -> Map.
 Parameter delete : Map -> k -> Map.
 
+
 Section WithRange.
+(* The environment initially chooses a type for the output of a hash 
+   function. *)
 Variable HRange : Set.
 
-Section WithDomain.
-(* Introduce a Domain for a hash function, as well as an instance
-   from Domain to Range. Define a Collision of two distinct elements
-   from the Domain with the same image in Range. *)
-Variable HDomain : Set.
-Variable h : HDomain -> HRange.
+(* Given an HRange, the implementation must provide instances for each 
+   of the following sets:
 
-Definition Collision := {ab | match ab with (a, b) => 
-                         a <> b /\ h a = h b end}.
+   HDomain: input to the hash function
+   Tree:    the entire data structure - O(N)
+   VO:      a path through a Tree (i.e., a Verification Object)used 
+            to verify a single operation - O(log N)
+   Digest:  a concise representation of a Tree - O(1)
+*)
 
-(* Define a family of monadic hash computations. We will provide
-   two instances of this family, each for a specific monad. *)
-Class HashComputation `{M0:Monad M} :=
-  hash_computation : HDomain -> M HRange.
+Class MerkleData := {
+  HDomain : Set;
+  Tree : Set;
+  VO : Set;
+  Digest : Set;
+  Empty : Tree
+}.
 
-(* The first instance of HashComputation runs in the identity monad.
-   The computation simply evaluates the hash function and returns 
-   the result. The monad scaffolding falls away, which is desirable
-   for correctness proofs. *)
-Instance HashIdC : HashComputation (M0:=IdentityMonad) := 
-  { hash_computation d := h d }.
+(* The implementation must also define several computations that
+   execute in a monad of the environment's choice. The implementation
+   has access only to the ordinary monadic composition 
+   operators (bind and return), as well as a HashComputation.
+   a number of computations in this Monad. *)
+Section WithData.
+Context (MD : MerkleData).
+Definition HashComputation (M:Type->Type) := HDomain -> M HRange.
 
-(* The second instance runs in a Counter monad (i.e., StateM nat). 
-   The computation evaluates the hash and returns it, but it also
-   increments the counter. For a worst-case complexity proof of 
-   a computation, it will suffice to bound the size of the counter
-   after the computation completes. *)
-Instance HashCountC : HashComputation (M0:=StateMonad nat) :=
-  { hash_computation d := fun c => (S c, h d) }.
-
-
-(* The computations must be defined for all Monads supporting a hash computation *)
-Class Computations M Digest VO Tree := {
+Class Computations (M:Type->Type) := {
 
     (* The _c computations take a full O(N) data structure (Tree) and
        return an O(log N) Verification Object (VO). The Server in a 
@@ -84,25 +68,35 @@ Class Computations M Digest VO Tree := {
     (* The _f are the  computations take a pair of VOs and produce a 
        Collision if the VOs result in conflicting answers when applied 
        to the corresponding _v. *)
-    search_f : Digest -> k -> VO -> VO -> M (option Collision);
-    insert_f : Digest -> k -> v -> VO -> VO -> M (option Collision);
-    delete_f : Digest -> k -> VO -> VO -> M (option Collision)
+    search_f : Digest -> k -> VO -> VO -> M (option (HDomain*HDomain));
+    insert_f : Digest -> k -> v -> VO -> VO -> M (option (HDomain*HDomain));
+    delete_f : Digest -> k -> VO -> VO -> M (option (HDomain*HDomain))
 }.
+Definition MerkleImpl := forall `{Monad M}, HashComputation M -> Computations M.
 
 
-Class MerkleComputations := {
-   Digest : Set;
-   VO : Set;
-   Tree : Set;
-   Empty : Tree;
+(* Given a MerkleImpl, which provides computations under any monad,
+   the algorithm requirements are expressed using two specific monads. *)
+Section MerkleSpec.
+Variable CC : MerkleImpl.
 
-   (* The computations must be defined over all monads with 
-      an available HashComputation *)
-   CC : forall M `{M0:Monad M} `{HC:HashComputation}, Computations M Digest VO Tree;
+Variable h : HDomain -> HRange.
+Definition Collision := {ab | match ab with (a, b) => 
+                         a <> b /\ h a = h b end}.
 
-   CCM := CC IdM (M0:=IdentityMonad) (HC:=HashIdC);
-   CountM := StateM nat;
-   CCC := CC CountM (M0:=StateMonad nat) (HC:=HashCountC);
+(* First, a trivial computation the Identity monad is used to express the 
+   functional correctness/security claims. *)
+Definition HashIdC : HashComputation IdM := fun d => h d.
+Definition CCM := CC IdM IdM_Me IdM_Return IdM_Bind IdentityMonad HashIdC.
+
+(* Second, a computation in the State monad that increments a counter is
+   used to express the complexity bounds. *)
+Definition CountM := StateM nat.
+Definition HashCountC : HashComputation CountM := fun d c => (S c, h d).
+Definition CCC := CC CountM (StateM_Me nat) (StateM_Return nat) (StateM_Bind nat)
+                  (StateMonad nat) HashCountC.
+
+Class MerkleSpec := {
 
 (* Requirement #1: Correctness *)
 (* Define a mapping from Trees to Maps. This is a homomorphism 
@@ -116,48 +110,50 @@ Class MerkleComputations := {
    T : Tree -> Map;
    T_empty : T Empty = empty;
 
-   digest : Tree -> Digest := fun t => digest_c (M:=IdM) t;
+   digest : Tree -> Digest := fun t => digest_c (Computations:=CCM) t;
 
-   search_T : forall t k, match search_c (M:=IdM) t k
+   search_T : forall t k, match search_c (Computations:=CCM) t k
               with vo =>
-                 search_v (M:=IdM) (digest t) k vo = Some (search (T t) k)
+                 search_v (Computations:=CCM) (digest t) k vo = Some (search (T t) k)
               end;
 
-   insert_T : forall t k v, match insert_c (M:=IdM) t k v
+   insert_T : forall t k v, match insert_c (Computations:=CCM) t k v
               with (vo, t') => 
                  T t' = insert (T t) k v
-              /\ insert_v (M:=IdM) (digest t) k v vo = Some (digest t')
+              /\ insert_v (Computations:=CCM) (digest t) k v vo = Some (digest t')
               end;
 
-   delete_T : forall t k, match delete_c (M:=IdM) t k
+   delete_T : forall t k, match delete_c (Computations:=CCM) t k
               with (vo, t') =>
                   T t' = delete (T t) k
-               /\ delete_v (M:=IdM) (digest t) k vo = Some (digest t')
+               /\ delete_v (Computations:=CCM) (digest t) k vo = Some (digest t')
               end;
 
+
 (* Requirement #2. Security *)
-(* If there are logical collisions in the tree, meaning a pair of VO's 
+(* If there is a logical collision in the tree, meaning a pair of VO's 
    that produce different outputs under search_v for some inputs, then
    the corresponding search_f will compute a Collision in the original
    hash function. *)
 
    search_F : forall d k vo vo' r r', 
                       r <> r'
-                   /\ search_v (M:=IdM) d k vo = Some r
-                   /\ search_v (M:=IdM) d k vo' = Some r' ->
-                      exists cc, search_f (M:=IdM) d k vo vo' = Some cc;
+                   /\ search_v (Computations:=CCM) d k vo = Some r
+                   /\ search_v (Computations:=CCM) d k vo' = Some r' ->
+                      exists cc, search_f (Computations:=CCM) d k vo vo' = Some cc;
 
    insert_F : forall d k v vo vo' r r', 
                       r <> r'
-                   /\ insert_v (M:=IdM) d k v vo = Some r
-                   /\ insert_v (M:=IdM) d k v vo' = Some r' ->
-                      exists cc, insert_f (M:=IdM) d k v vo vo' = Some cc;
+                   /\ insert_v (Computations:=CCM) d k v vo = Some r
+                   /\ insert_v (Computations:=CCM) d k v vo' = Some r' ->
+                      exists cc, insert_f (Computations:=CCM) d k v vo vo' = Some cc;
 
    delete_F : forall d k vo vo' r r', 
                       r <> r'
-                   /\ delete_v (M:=IdM) d k vo = Some r
-                   /\ delete_v (M:=IdM) d k vo' = Some r' ->
-                      exists cc, delete_f (M:=IdM) d k vo vo' = Some cc;
+                   /\ delete_v (Computations:=CCM) d k vo = Some r
+                   /\ delete_v (Computations:=CCM) d k vo' = Some r' ->
+                      exists cc, delete_f (Computations:=CCM) d k vo vo' = Some cc;
+
 
 (* Requirement #3. Complexity *)
 (* All of the computations must run in O(poly N) time. When each
@@ -167,19 +163,23 @@ Class MerkleComputations := {
 
    polybound : nat -> nat;
 
-   search_c_C : forall t k, match search_c (M:=StateM nat) t k 0
+   search_c_C : forall t k, match search_c (Computations:=CCC) t k 0
                      with (c, _) => c <= polybound (size (T t)) end;
-   insert_c_C : forall t k v, match insert_c (M:=StateM nat) t k v 0
+   insert_c_C : forall t k v, match insert_c (Computations:=CCC) t k v 0
                      with (c, _) => c <= polybound (size (T t)) end;
-   delete_c_C : forall t k, match delete_c (M:=StateM nat) t k 0
+   delete_c_C : forall t k, match delete_c (Computations:=CCC) t k 0
                      with (c, _) => c <= polybound (size (T t)) end
 }.
-End WithDomain.
-
-Class MerkleInstance := {
-   HDomain : Set;
-   MI : forall h : HDomain -> HRange, MerkleComputations HDomain h
-}.
+End MerkleSpec.
+End WithData.
 End WithRange.
 
+
+Record MerkleInstance (HRange:Set) := {
+   Types : MerkleData;
+   Implementation : MerkleImpl HRange Types;
+   Proofs : forall h : HDomain -> HRange, MerkleSpec HRange Types Implementation h
+}.
+
+(* Finally, this is the overall type of satisfactory solutions. *)
 Definition MerkleSolution := forall HRange, MerkleInstance HRange.
